Make progress on the mutator in min+max
The mutator now calls the two separate mutators from the min&max and
the spec implementation.  However, it has some very unfortunate
constructs, like

  x <- { _ : { x : A | computes_to bar x } | True };
  ...

This is necessary to generate (inside the computation monad) the proof
that the the [x] which [bar] computes to satisfies some properties,
which mention [bar].  I suspect that I'll be able to remove these
constructs later in the refinement process, when I figure out how to
say that you can strip off the proof part of a [sig] representation if
it's only ever used to compute the proof part of a mutator.  But I
don't think I can hide all the details behind the "general delegation
refinement".

I kind-of want to thread the proofs through variants of, e.g., [Pick],
so that we can get [Comp] support for this.  Alternatively, I kind-of
want to build the representation invariants into the ADT structure, so
we don't have to use the proofs in the [Comp].  But there might be
another better way to do this, that I'm not seeing.

ADTExamples/MinPlusMax.v
@@ -28,16 +28,66 @@ Section MinMaxExample.
 
   Variable MinMaxImpl : ADT MinMaxSig.
   Variable refineMinMax : refineADT MinMaxSpec MinMaxImpl.
+  Let SiR := SiR refineMinMax.
 
   Definition MinMaxSiR (or : multiset) (nr : Rep MinMaxImpl) :=
-    exists SiR : multiset -> Rep MinMaxImpl -> Prop,
-      SiR or nr /\
-      (forall idx : ObserverIndex MinMaxSig,
-         refineObserver SiR (ObserverMethods MinMaxSpec idx)
-                        (ObserverMethods MinMaxImpl idx)) /\
-      (forall idx : MutatorIndex MinMaxSig,
-         refineMutator SiR (MutatorMethods MinMaxSpec idx)
-                       (MutatorMethods MinMaxImpl idx)).
+    SiR or nr.
+
+  Lemma refineObserver_MinMaxSiR
+  : forall idx : ObserverIndex MinMaxSig,
+      refineObserver SiR (ObserverMethods MinMaxSpec idx)
+                     (ObserverMethods MinMaxImpl idx).
+  Proof.
+    destruct refineMinMax; eauto.
+  Qed.
+  Lemma refineMutator_MinMaxSiR
+  : forall idx : MutatorIndex MinMaxSig,
+      refineMutator SiR (MutatorMethods MinMaxSpec idx)
+                    (MutatorMethods MinMaxImpl idx).
+  Proof.
+    destruct refineMinMax; eauto.
+  Qed.
+
+  Hypothesis refineMutatorPreservesSiR
+  : forall idx : MutatorIndex MinMaxSig,
+      forall x0 k x1 x2 y,
+        computes_to (MutatorMethods MinMaxSpec idx x0 k) x1
+        -> computes_to (MutatorMethods MinMaxSpec idx x0 k) x2
+        -> SiR x1 y
+        -> SiR x2 y.
+
+  Lemma helper_SiR_preserved
+        (r : {nr : multiset * Rep MinMaxImpl | MinMaxSiR (fst nr) (snd nr)})
+        (x : nat)
+        (r1 : {v : multiset | {m' : multiset | add_spec (fst (` r)) x m'} ↝ v})
+        (r2 : {v : Rep MinMaxImpl |
+               (callMut MinMaxImpl "Insert") (snd (` r)) x ↝ v})
+  : MinMaxSiR (` r1) (` r2).
+  Proof.
+    unfold MinMaxSiR in *.
+    pose proof (refineMutatorPreservesSiR {| bstring := "Insert" |}) as SiRPreserved.
+    clear refineMutatorPreservesSiR; simpl in *.
+    abstract (
+        destruct_head sig;
+        simpl in *;
+          inversion_by computes_to_inv;
+        let H := fresh in
+        pose proof (refineMutator_MinMaxSiR {| bstring := "Insert" |}) as H;
+        simpl in *;
+          match goal with
+            | [ x : _, y : _, z : _ |- _ ] =>
+              specialize (H _ _ x y _ z)
+          end;
+        repeat match goal with
+                 | [ H : computes_to _ _ |- _ ] => apply computes_to_inv in H
+                 | _ => progress destruct_head ex
+                 | _ => progress destruct_head and
+               end;
+        eapply SiRPreserved;
+        solve [ eassumption
+              | constructor; eassumption ]
+      ).
+  Qed.
   (*
   Inductive type_SiR {Sig} {A B : ADT Sig} (P : (Rep A -> Rep B -> Prop) -> Prop) : refineADT A B -> Type
     := Build_type_SiR : forall SiR H0 H1,
@@ -221,8 +271,11 @@ Section MinMaxExample.
       let H' := fresh "H'" in
       lazymatch goal with
         | [ r_n : sig _ |- _ ]
-          => destruct (proj2_sig r_n) as [SiR [H [H' ?]]];
-            specialize (fun arg => H' {| bstring := rew_observer_name |} _ _ arg H);
+          => pose proof (fun arg =>
+                           refineObserver_MinMaxSiR
+                             {| bstring := rew_observer_name |}
+                             _ _ arg
+                             (proj2_sig r_n)) as H';
             simpl in H';
             set_evars;
             instantiate;
@@ -252,212 +305,36 @@ Section MinMaxExample.
     (** Rewrite the "Min" and then "Max" [Pick] in the MinPlusMax Observer. *)
     dubiously specialized hone ∑-observer "MinPlusMax"%string  rewriting with observer "Min"%string.
     dubiously specialized hone ∑-observer "MinPlusMax"%string  rewriting with observer "Max"%string.
-    hone'' ∑-mutator "Insert"%string.
+    hone'' ∑-mutator "Insert"%string using
+           (fun (r : {nr : multiset * Rep MinMaxImpl | MinMaxSiR (fst nr) (snd nr)}) x =>
+              (r1 <- { v : { v | callMut MinPlusMaxSpec "Insert" (fst (proj1_sig r)) x ↝ v } | True };
+               r2 <- { v : { v | callMut MinMaxImpl "Insert" (snd (proj1_sig r)) x ↝ v } | True};
+               ret (exist (fun nr => MinMaxSiR (fst nr) (snd nr)) (`r1, `r2) (helper_SiR_preserved _ r1 r2) ))).
     { intros.
       subst.
-      set_evars; simpl in *.
-      unfold two_op_spec.
       unfold delegateADTSiR; simpl.
       setoid_rewrite remove_forall_eq0.
       setoid_rewrite remove_exists_and_eq0.
       setoid_rewrite refineEquiv_pick_eq'.
       autorewrite with refine_monad.
-      subst_body.
-      higher_order_2_reflexivity. }
-     (*
-      destruct refineMinMax.
-      SearchAbout refineEquiv Pick eq.
-      setoid_rewrite refineEquiv_pick_computes_to.
-      setoid_rewrite refineEquiv_split_func_ex2'.
-      subst_body.
-      rewrite_hyp.
-      simpl in *.
-      unfold delegateADTSiR; simpl; subst.
-      set_evars.
-      lazymatch goal with |- refine _ (?f _ _) => is_evar f; set (H' := f) end.
-      setoid_rewrite remove_forall_eq0.
-      se
-    (* TODO: Implement the Insert Mutator. *)
-    (*** HERE *)
-    (** Idea: do it the same way we split out the picks in the observer *)
-    hone'' mutator "Insert"%string using
-          (fun (r : {nr : multiset * Rep MinMaxImpl | MinMaxSiR (fst nr) (snd nr)}) x =>
-             r1 <- callMut MinPlusMaxSpec "Insert" (fst (proj1_sig r)) x;
-           r2 <- callMut MinMaxImpl "Insert" (snd (proj1_sig r)) x;
-           ret (ex_intro (fun nr => MinMaxSiR (fst nr) (snd nr)) (r1, r2) _ )).
-    intros; subst.
-    simpl.
-    - destruct extract_MinMaxSiR as [MinMaxSiR [refineMinMaxObs refineMinMaxMut] ].
-      eapply refineADT_BuildADT_Rep with
-      (SiR := fun (or nr : Rep MinPlusMaxSpec * Rep MinMaxImpl) =>
-                or = nr /\
-                MinMaxSiR (fst nr) (snd nr)).
-      unfold getMutDef; simpl; unfold ith_obligation_2; simpl.
-      intros mutIdx r_o r_n; find_if_inside; intros; intuition;
-      subst; simpl; autorefine.
-      unfold refine; intros; inversion_by computes_to_inv; subst;
-      econstructor.
-      econstructor; intros; subst; eexists; split.
-      econstructor; eauto.
-      instantiate (1 := (x, x0)); reflexivity.
-      econstructor; split; eauto.
-      generalize (refineMinMaxMut {| bounded_s := "Insert"%string |} _ _ n H1 _ H2);
-        simpl; unfold getMutDef; simpl; intros.
-      inversion_by computes_to_inv; unfold add_spec in *.
-      assert (x1 = x) by
-          (apply functional_extensionality;
-           intros; rewrite H0, H3; reflexivity).
-      rewrite H in H4; assumption.
-      intros; unfold refineObserver; intros; intuition; subst;
-      reflexivity.
-    - (** Implement the MinPlusMax Observer. *)
-      hone'' observer "MinPlusMax"%string.
-      Print refineADT.
-      (** TODO: Write small manual inversion tactic to pick up hypothesis automatically *)
-      inversion_clear refineMinMax.
-      exists (fun a b => fst a = fst b /\ SiR (fst a) (snd a) /\ SiR (fst b) (snd b)).
-      unfold ith_obligation_2 in *; simpl in *.
-      repeat split; intros; simpl.
-      specialize (H {| bounded_s := "Insert" |}).
-      pose proof (H0 {| bounded_s := "Min" |}) as H0'.
-      specialize (H0 {| bounded_s := "Max" |}).
-      revert H H0 H0'.
-      simpl.
-      find_if_inside; simpl.
+      eapply refine_pick.
       intros.
-      split_and; destruct_head prod; subst.
-      repeat (setoid_rewrite refineEquiv_bind_bind || setoid_rewrite refineEquiv_bind_unit || setoid_rewrite refineEquiv_unit_bind).
-      simpl in *.
-      eapply refine_bind; [ reflexivity | intro ].
-      (** HERE *)
-
-      admit.
-      admit.
-      admit.
-
-
-      unfold two_op_spec.
-
-
-      setoid_rewrite remove_forall_eq'.
-
-
-
-
-      repeat setoid_rewrite refineEquiv_bind_bind.
-      repeat setoid_rewrite
-      autorewrite with refine_monad.
-let P := match goal with |- ex ?P => constr:(P) end in
-      refine (match refineMinMax in (return ex P with
-                | @refinesADT _ _ SiR _ _ => ex_intro P SiR _
-              end).
-
-      let G := match goal with |- ?G => constr:(G) end in
-      pose (fun SiR => (@refineADT_BuildADT_ReplaceObserver_generic _ _ _ _ _ {| bounded_s := "MinPlusMax"%string |} _ _ SiR _ _: G)).
-      Print refineADT.
-      match refineMinMax return (
-           (fun (r : Rep MinPlusMaxSpec * Rep MinMaxImpl)
-                n =>
-              (min <- (ObserverMethods MinMaxImpl
-                                       {|bounded_s := "Min"%string |} (snd r) n);
-               max <- (ObserverMethods MinMaxImpl
-                                       {|bounded_s := "Max"%string |} (snd r) n);
-               ret ((min + max)))%comp).
-    destruct extract_MinMaxSiR as [MinMaxSiR [refineMinMaxObs refineMinMaxMut] ].
-    eapply refineADT_BuildADT_Rep with
-    (SiR := fun (or nr : Rep MinPlusMaxSpec * Rep MinMaxImpl) =>
-              or = nr /\
-              MinMaxSiR (fst nr) (snd nr)).
-    Focus 2.
-    unfold getObsDef; simpl; intros.
-
-
-    eapply SharpenStep with (adt' :=
-                               {|
-     Rep := Rep MinPlusMaxSpec * Rep MinMaxImpl;
-     MutatorMethods := fun
-                         (idx : MutatorIndex
-                                  (CombTwoOpCollectionSig "MinPlusMax"))
-                         (r : Rep MinPlusMaxSpec * Rep MinMaxImpl)
-                         (x : MutatorDom
-                                (CombTwoOpCollectionSig "MinPlusMax") idx) =>
-                        r1 <- MutatorMethods MinPlusMaxSpec idx (fst r) x;
-     r2 <- MutatorMethods MinMaxImpl idx (snd r) x;
-                       ret (r1, r2);
-     ObserverMethods := fun
-                         (idx : ObserverIndex
-                                  (CombTwoOpCollectionSig "MinPlusMax"))
-                         (r : Rep MinPlusMaxSpec * Rep MinMaxImpl)
-                         n =>
-                         (min <- (ObserverMethods MinMaxImpl
-                                                  {|bounded_s := "Min"%string |} (snd r) (foo _ n));
-                          max <- (ObserverMethods MinMaxImpl
-                                                  {|bounded_s := "Max"%string |} (snd r) (foo _ n));
-                          ret (bar idx (min + max)))%comp |}).
-    assert (exists SiR : multiset -> Rep MinMaxImpl -> Prop,
-              (forall idx : ObserverIndex MinMaxSig,
-                refineObserver SiR (ObserverMethods MinMaxSpec idx)
-                               (ObserverMethods MinMaxImpl idx)) /\
-              (forall idx : MutatorIndex MinMaxSig,
-                  refineMutator SiR (MutatorMethods MinMaxSpec idx)
-                                 (MutatorMethods MinMaxImpl idx))).
-    inversion refineMinMax; eauto.
-    clear refineMinMax; destruct H as [SiR [refineMinMaxObs refineMinMaxMut] ].
-    eapply refineADT_Build_ADT_Rep with
-    (SiR := fun (or nr : Rep MinPlusMaxSpec * Rep MinMaxImpl) =>
-              or = nr /\
-              SiR (fst nr) (snd nr)).
-    - intro.
-      assert (exists pf,
-                mutIdx = {| bounded_s := "Insert"%string;
-                            s_bounded := pf |}) as mutIdx_eq by
-          (clear;
-           destruct mutIdx; destruct s_bounded; inversion sbound;
-           subst; simpl;
-           [ exists {| sbound := sbound |}; reflexivity
-                  | inversion H ]) ;
-      destruct mutIdx_eq as [pf mutIdx_eq]; rewrite mutIdx_eq.
-      unfold refineMutator; intros; intuition; subst.
-      unfold refine; intros; econstructor; eauto.
-      econstructor; split; eauto.
-      inversion_by computes_to_inv; subst; simpl.
-      generalize (refineMinMaxMut _  _ _ n H1 _ H2); intros.
+      constructor.
       inversion_by computes_to_inv.
-      unfold getMutDef in H0, H3; simpl in H0, H3.
+      subst; simpl.
+      destruct_head sig.
       inversion_by computes_to_inv.
-      unfold add_spec in *.
-      assert (x1 = x) by
-          (apply functional_extensionality;
-           intros; rewrite H0, H3; reflexivity).
-      rewrite H in H4; assumption.
-    - intro;
-      assert (exists pf,
-                 obsIdx = {| bounded_s := "MinPlusMax"%string;
-                            s_bounded := pf |}) as obsIdx_eq by
-          (clear;
-           destruct obsIdx; destruct s_bounded; inversion sbound;
-           subst; simpl;
-           [ exists {| sbound := sbound |}; reflexivity
-                  | inversion H ]) ;
-      destruct obsIdx_eq as [pf obsIdx_eq]; rewrite obsIdx_eq.
-      simpl; intros; intuition; subst; unfold getObsDef; simpl.
-      unfold two_op_spec, refine; intros.
-      apply computes_to_inv in H; destruct_ex; intuition.
-      apply computes_to_inv in H2; destruct_ex; intuition.
-      apply computes_to_inv in H3; destruct_ex; intuition.
-      destruct pf; subst.
-      econstructor; eexists x; split; eauto.
-      generalize (refineMinMaxObs {|bounded_s := "Min" |} _ _ _ H1 _ H0).
-      simpl; unfold getObsDef; simpl; intros; inversion_by computes_to_inv; eauto.
-      eexists x0; split; eauto.
-      generalize (refineMinMaxObs {|bounded_s := "Max" |} _ _ _ H1 _ H2).
-      simpl; unfold getObsDef; simpl; intros; inversion_by computes_to_inv; eauto. *)
+      trivial. }
     - finish sharpening.
   Defined.
 
   (* Show the term derived above as a sanity check. *)
   Goal (forall b, ObserverMethods (projT1 (MinPlusMaxImpl 0))
                                  {| bstring := "MinPlusMax" |} = b).
+    simpl.
+  Abort.
+  Goal (forall b, MutatorMethods (projT1 (MinPlusMaxImpl 0))
+                                 {| bstring := "Insert" |} = b).
     simpl.
   Abort.
 
